theories/ub_logic/merkle/unreliable.v
@@ -98,30 +98,13 @@ Section unreliable_storage.
       ("l", merkle_tree_decider_program val_bit_size' "hash" "lhmf").
   
 
-  Inductive tree_leaf_list: nat -> merkle_tree -> list nat -> Prop :=
-  | tree_leaf_list_lf h lf: tree_leaf_list 0 (Leaf h lf) (lf::[])
-  | tree_leaf_list_br n a alist b blist h:
-    tree_leaf_list n a alist ->
-    tree_leaf_list n b blist ->
-    tree_leaf_list (S n) (Branch h a b) (alist ++ blist).
-
-  Lemma tree_leaf_list_length n tree lis:
-    tree_leaf_list n tree lis -> length lis = 2^n.
-  Proof.
-    revert tree lis.
-    induction n; intros tree lis Hlist.
-    - inversion Hlist. by simpl.
-    - inversion Hlist; subst. rewrite app_length. simpl. erewrite !IHn; try done.
-      lia.
-  Qed.
 
   Lemma tree_builder_helper_spec (list:list nat) (vlist: val) (height:nat) (m:gmap nat Z) (f:val):
     size (m) + 2^(S height) - 1 <= max_hash_size ->
     length list = 2^height ->
     Forall (λ x, x < 2^(2*val_bit_size)) list ->
     is_list list vlist ->
-    {{{ hashfun_amortized val_size_for_hash max_hash_size f m ∗
-        ⌜coll_free m⌝ ∗
+    {{{ coll_free_hashfun_amortized val_size_for_hash max_hash_size f m ∗
         € (nnreal_nat (2^(S height)-1) * amortized_error val_size_for_hash max_hash_size)%NNR
     }}}
       tree_builder_helper f #height vlist 
@@ -129,15 +112,14 @@ Section unreliable_storage.
           ∃ (m':gmap nat Z) (tree:merkle_tree),
             ⌜m ⊆ m'⌝ ∗
             ⌜size (m') <= size (m) + 2^(S height) - 1⌝ ∗
-            hashfun_amortized val_size_for_hash max_hash_size f m' ∗
-            ⌜coll_free m'⌝ ∗
+            coll_free_hashfun_amortized val_size_for_hash max_hash_size f m' ∗
             ⌜tree_leaf_list height tree list⌝ ∗
             ⌜tree_valid val_bit_size' height tree m'⌝ ∗
             ⌜root_hash_value tree = hash ⌝
       }}}.
   Proof.
-    iIntros (Hmsize Hlength Hforall Hislist Φ) "(H&%Hcollfree&Herr) HΦ".
-    iInduction height as [|height] "IH" forall (list vlist m Hmsize Hlength Hforall Hislist Φ Hcollfree).
+    iIntros (Hmsize Hlength Hforall Hislist Φ) "(H&Herr) HΦ".
+    iInduction height as [|height] "IH" forall (list vlist m Hmsize Hlength Hforall Hislist Φ).
     - rewrite /tree_builder_helper. wp_pures.
       assert (∃ x:nat, list = x::[]) as [x ->].
       { destruct list as [| ? [|]]; first done.
@@ -150,24 +132,16 @@ Section unreliable_storage.
       wp_pures.
       wp_apply (wp_insert_amortized with "[$H Herr]").
       + simpl in Hmsize. lia.
-      + iSplitL; last done.
-        iApply ec_spend_irrel; last done.
+      + iApply ec_spend_irrel; last done.
         simpl. lra.
-      + iIntros (hash) "(%m' & H&%&%&%&%)".
+      + iIntros (hash) "(%m' & H&%&%&%)".
         wp_pures. replace 2%Z with (Z.of_nat 2) by lia.
         wp_apply unreliable_alloc_spec; [lia|done|].
         iIntros (l) "_".
         wp_pures.
         iAssert (⌜(0<=hash<2^val_bit_size)%Z⌝)%I as "[%Ha %Hb]".
-        { iDestruct "H" as "(%&%&%&%&%K' &H)".
-          iPureIntro.
-          eapply map_Forall_lookup_1 in K' as [? K']; last done.
-          split; try lia.
-          rewrite /val_size_for_hash in K'. rewrite Z.lt_le_pred.
-          eapply Z.le_stepr; first done.
-          rewrite Nat2Z.inj_sub; last first.
-          - clear. induction val_bit_size; simpl; lia.
-          - rewrite Nat2Z.inj_pow. lia. 
+        { iPoseProof (coll_free_hashfun_amortized_implies_bounded_range with "[$H][//]") as "[% %T]".
+          iPureIntro. by apply hash_bound_manipulation.
         }
         replace (hash) with (Z.of_nat $ Z.to_nat hash); last lia.
         wp_apply unreliable_write_spec; first done.
@@ -179,9 +153,9 @@ Section unreliable_storage.
         iModIntro.
         iApply "HΦ".
         iExists m', _.
-        repeat iSplit; try done.
+        repeat (try iSplit; try done).
         * iPureIntro. simpl; lia.
-        * iPureIntro; constructor.
+        * iPureIntro. constructor.
         * iPureIntro; constructor.
           -- instantiate (1 := Z.to_nat hash).
              rewrite /merkle_tree.val_bit_size.
@@ -216,21 +190,21 @@ Section unreliable_storage.
       }
       subst.
       replace (Z.of_nat (S height) - 1)%Z with (Z.of_nat height); last lia.
-      wp_apply ("IH" with "[][][][][][$H][$Herr]"); try iPureIntro; try done.
+      wp_apply ("IH" with "[][][][][$H][$Herr]"); try iPureIntro; try done.
       + assert (2^S height <= 2^ S (S height)); try lia.
         simpl. lia.
       + by apply Forall_app in Hforall as [Hforall1 Hforall2].
-      + iIntros (hasha la) "(%m' & %treea & %&%&H&%&%&%&%)".
+      + iIntros (hasha la) "(%m' & %treea & %&%&H&%&%&%)".
         wp_pures.
         replace (Z.of_nat (S height) - 1)%Z with (Z.of_nat height); last lia.
-        wp_apply ("IH"$! l2 with "[][][][][][$H][$Herr']"); try iPureIntro; try done.
+        wp_apply ("IH"$! l2 with "[][][][][$H][$Herr']"); try iPureIntro; try done.
         * trans (size m + 2^ S height - 1 + 2 ^ S height - 1); try lia.
           etrans; last exact. simpl. lia.
         * replace (2^ S height) with (2^height + 2 ^ height) in Hlength; last first.
           { simpl. lia. }
           rewrite app_length in Hlength. lia.
         * rewrite Forall_app in Hforall. set_solver.
-        * iIntros (hashb lb) "(%m'' & %treeb & %&%&H&%&%&%&%)".
+        * iIntros (hashb lb) "(%m'' & %treeb & %&%&H&%&%&%)".
           wp_pures.
           wp_apply pow_spec; first done.
           iIntros (?) "->".
@@ -242,24 +216,17 @@ Section unreliable_storage.
              apply (PeanoNat.Nat.le_lt_trans _ (size m + 2 ^ S height - 1 + 2^S height - 1)); try lia.
              clear. simpl. assert (0<2^height); try lia.
              induction height; simpl; lia.
-          -- iSplit; last done. iApply ec_spend_irrel; last done.
+          -- iApply ec_spend_irrel; last done.
              simpl. lra.
-          -- iIntros (hash) "(%m''' & H&%&%Hfound&%&%)".
+          -- iIntros (hash) "(%m''' & H&%Hfound&%&%)".
              wp_pures.
              replace 3%Z with (Z.of_nat 3) by lia.
              wp_apply unreliable_alloc_spec; [lia|done|].
              iIntros (?) "_".
              wp_pures.
              iAssert (⌜(0<=hash<2^val_bit_size)%Z⌝)%I as "[%Ha %Hb]".
-             { iDestruct "H" as "(%&%&%&%&%K' &H)".
-               iPureIntro.
-               eapply map_Forall_lookup_1 in K' as [? K']; last done.
-               split; try lia.
-               rewrite /val_size_for_hash in K'. rewrite Z.lt_le_pred.
-               eapply Z.le_stepr; first done.
-               rewrite Nat2Z.inj_sub; last first.
-               - clear. induction val_bit_size; simpl; lia.
-               - rewrite Nat2Z.inj_pow. lia. 
+             { iPoseProof (coll_free_hashfun_amortized_implies_bounded_range with "[$H][//]") as "[% %T]".
+               iPureIntro. by apply hash_bound_manipulation.
              }
              replace (hash) with (Z.of_nat (Z.to_nat hash)); last lia.
              wp_apply unreliable_write_spec; first done.
@@ -275,7 +242,7 @@ Section unreliable_storage.
              wp_pures.
              iModIntro. iApply "HΦ".
              iExists m''', (Branch (Z.to_nat hash) treea treeb).
-             repeat iSplit; try done.
+             repeat (try iSplit; try done).
              ++ iPureIntro. by do 3 (etrans; last exact).
              ++ iPureIntro. replace (_+_-_) with (size m + 2 ^ S height + 2^ S height - 1); last by (simpl;lia).
                 trans (size m' + 2^S height); last lia.
@@ -309,9 +276,8 @@ Section unreliable_storage.
       tree_builder vlist #height
       {{{ (l:nat) (checker:val), RET (#l, checker);
           ∃ (m:gmap nat Z) (tree:merkle_tree) (f:val),
-            hashfun_amortized val_size_for_hash max_hash_size f m ∗
+            coll_free_hashfun_amortized val_size_for_hash max_hash_size f m ∗
             ⌜tree_valid val_bit_size' height tree m⌝ ∗
-            ⌜coll_free m⌝ ∗
             ⌜size (m) <= 2^(S height) - 1⌝ ∗
             ⌜tree_leaf_list height tree list⌝ ∗
             decider_program_helper_spec height val_bit_size' max_hash_size checker tree f
@@ -321,11 +287,10 @@ Section unreliable_storage.
     rewrite /tree_builder.
     wp_pures.
     wp_apply (wp_init_hash_amortized _ max_hash_size); first done.
-    iIntros (f) "H".
+    iIntros (f) "H". iMod "H".
     wp_pures.
     wp_apply (tree_builder_helper_spec with "[$H $Herr]"); [done|done|done|done|..].
-    { iPureIntro. intros ???H??. exfalso. destruct H. set_solver. }
-    iIntros (hash l) "(%m'&%tree&%&%&H&%&%&%&%Hhash)".
+    iIntros (hash l) "(%m'&%tree&%&%&H&%&%&%Hhash)".
     wp_pures. rewrite <-Hhash.
     wp_apply (merkle_tree_decider_program_spec with "[$H]").
     - done. 
@@ -333,7 +298,7 @@ Section unreliable_storage.
       wp_pures.
       iApply "HΦ".
       iModIntro.
-      iExists _,_,_. by repeat iSplit. 
+      iExists _,_,_. iFrame. by repeat iSplit. 
   Qed.
   
   (** looking up the tree *)
@@ -365,62 +330,6 @@ Section unreliable_storage.
       if: list_forall proof_bound_checker "proof" && (#0 < "leaf") && ("leaf" < #(2^(val_bit_size*2)))
       then if: "checker" "proof" "leaf" then (SOME "leaf") else NONEV
       else NONEV.
-
-  Inductive proof_idx_relate : nat -> list (bool*nat) -> nat -> Prop :=
-  | proof_idx_relate_lf: proof_idx_relate 0 [] 0
-  | proof_idx_relate_left idx n rhash proof:
-    proof_idx_relate n proof idx ->
-    idx < 2^n -> 
-    proof_idx_relate (S n) ((true, rhash)::proof) idx
-  | proof_idx_relate_right idx n lhash proof:
-      proof_idx_relate n proof (idx - 2^n) ->
-      2^n <= idx ->
-      proof_idx_relate (S n) ((false, lhash)::proof) idx
-  .
-
-  Lemma proof_idx_relate_implies_possible_proof tree proof height idx m:
-    tree_valid val_bit_size' height tree m ->
-    proof_idx_relate height proof idx ->
-    Forall (λ x : bool * nat, x.2 < 2 ^ val_bit_size) proof ->
-    possible_proof val_bit_size' tree proof.
-  Proof.
-    revert tree proof idx.
-    induction height; intros tree proof idx Htvalid Hrelate Hforall.
-    - inversion Hrelate; inversion Htvalid; subst. constructor.
-    - inversion Htvalid; inversion Hrelate; subst.
-      + constructor.
-        * eapply IHheight; try done. by eapply Forall_inv_tail.
-        * by apply Forall_inv in Hforall.
-      + constructor.
-        * eapply IHheight; try done. by eapply Forall_inv_tail.
-        * by apply Forall_inv in Hforall.
-  Qed.
-
-  
-  Lemma tree_leaf_list_implies_lookup_some lis tree height proof idx leafv:
-    tree_leaf_list height tree lis ->
-    proof_idx_relate height proof idx ->
-    tree_leaf_value_match tree leafv proof ->
-    lis !! idx = Some leafv. 
-  Proof.
-    revert lis tree proof idx leafv.
-    induction height as [|height]; intros lis tree proof idx leafv Hlist Hrelate Hmatch.
-    - inversion Hrelate; inversion Hmatch; subst; try done.
-      by inversion Hlist; subst.
-    - inversion Hrelate; subst.
-      + inversion Hrelate; inversion Hmatch; inversion Hlist; subst.
-        assert (length alist = 2^height).
-        { by eapply tree_leaf_list_length. }
-        rewrite lookup_app_l; last lia.
-        naive_solver.
-      + inversion Hrelate; inversion Hmatch; inversion Hlist; subst.
-        assert (length alist = 2^height) as K.
-        { by eapply tree_leaf_list_length. }
-        rewrite lookup_app_r; last lia.
-        rewrite K.
-        naive_solver.
-  Qed.
-
 
   Lemma tree_lookup_helper_spec (ltree:nat) (height:nat) (idx:nat):
     idx < 2^height -> 
@@ -531,8 +440,7 @@ Section unreliable_storage.
     {{{ decider_program_helper_spec height val_bit_size' max_hash_size checker tree f ∗
         ⌜tree_leaf_list height tree lis⌝ ∗
         ⌜tree_valid val_bit_size' height tree m⌝ ∗
-        hashfun_amortized val_size_for_hash max_hash_size f m ∗
-        ⌜coll_free m⌝ ∗
+        coll_free_hashfun_amortized val_size_for_hash max_hash_size f m ∗
         ⌜size (m) + S height <= max_hash_size⌝ ∗
         € ((nnreal_nat (S height)) * amortized_error val_size_for_hash max_hash_size)%NNR              
     }}}
@@ -541,7 +449,7 @@ Section unreliable_storage.
           ⌜∀ x:nat, v=SOMEV #x -> lis!!idx = Some x⌝
       }}}.
   Proof.
-    iIntros (Hidx Φ) "(#Hdecider & %Htreelist & %Htvalid & H & %Hmvalid & %Hmsize & Herr) HΦ".
+    iIntros (Hidx Φ) "(#Hdecider & %Htreelist & %Htvalid & H & %Hmsize & Herr) HΦ".
     rewrite /tree_lookup.
     wp_pures.
     wp_apply tree_lookup_helper_spec; [done|done|].
